Semi-automatic way to get good TCs from monadic definitions
Automating the steps taken by Konrad in HOL's
src/tfl/examples/monad.cong, using conversions for (inverse) eta
conversion on selected constants.

hol/reduceScript.sml
@@ -2,15 +2,315 @@ open HolKernel boolLib bossLib Parse monadsyntax ptypes_definitionsTheory lcsymt
 
 val _ = new_theory "reduce"
 
-val foo_def = tDefine "foo"`
-  foo M =
+(*
+val STATE_OPTION_IGNORE_BIND_weak_cong = Q.store_thm(
+"STATE_OPTION_IGNORE_BIND_weak_cong",
+`(m1 = m1') ∧
+ (!s''. (∃s. OPTION_MAP SND (m1' s) = SOME s'') ⇒ (m2 s'' = m2' s'')) ⇒
+ (STATE_OPTION_IGNORE_BIND m1 m2 = STATE_OPTION_IGNORE_BIND m1' m2')`,
+srw_tac [boolSimps.DNF_ss][STATE_OPTION_IGNORE_BIND_def,FUN_EQ_THM] >>
+Cases_on `m1' x` >> srw_tac [][] >> PROVE_TAC []);
+val () = DefnBase.add_cong STATE_OPTION_IGNORE_BIND_weak_cong;
+(* fix drop_cong if there are going to be multiple congruences... *)
+
+val STATE_OPTION_BIND_weak_cong = Q.store_thm(
+"STATE_OPTION_BIND_weak_cong",
+`(m = m') ∧
+ (∀v s''. (∃s. (m' s = SOME (v,s''))) ⇒ (f v s'' = f' v s'')) ⇒
+ (STATE_OPTION_BIND m f = STATE_OPTION_BIND m' f')`,
+srw_tac [boolSimps.DNF_ss][STATE_OPTION_BIND_def,FUN_EQ_THM] >>
+Cases_on `m' x` >> srw_tac [][pairTheory.UNCURRY] >>
+first_x_assum match_mp_tac >> srw_tac [][pairTheory.EXISTS_PROD] >>
+PROVE_TAC [] );
+val () = DefnBase.add_cong STATE_OPTION_BIND_weak_cong;
+*)
+
+(*
+val tm = ``foo a1 a2``
+val (rator,rand) = dest_comb tm
+val th = SIMP_CONV pure_ss [Ntimes (GSYM BETA_THM) 2] ``bar a1 a2 a3``;
+
+val INVERSE_ETA_THM = save_thm(
+"INVERSE_ETA_THM",
+FUN_EQ_THM |>  Q.SPEC `f` |> Q.SPEC `\x. f x` |> EQ_IMP_RULE |> snd
+|> UNDISCH |> PROVE_HYP (BETA_THM |> GSYM |> Q.SPEC `f`)
+|> Q.GEN `f`);
+
+val th1 = 
+((RATOR_CONV (SIMP_CONV pure_ss [Once INVERSE_ETA_THM])) THENC
+(fn tm => RATOR_CONV (ALPHA_CONV (snd(dest_comb tm))) tm))
+``bar a1``
+
+val th2 =
+((RATOR_CONV (SIMP_CONV pure_ss [Once INVERSE_ETA_THM])) THENC
+(fn tm => RATOR_CONV (ALPHA_CONV (snd(dest_comb tm))) tm))
+``bar a1 a2``
+
+SIMP_CONV pure_ss [Once th1] ``bar a1 a2``
+INVERSE_ETA_THM
+th2
+SUBS [th1] th2
+SUBS_OCCS [([2],th1)] th2
+GSYM (SUBST_MATCH th1 (GSYM th2))
+
+ONCE_REWRITE_RULE [th1] th2
+help"SUBS_OCCS";
+
+CONV_RULE BETA_CONV it
+help"SimpRHS"
+
+CONV_RULE (RAND_CONV (ONCE_DEPTH_CONV ETA_CONV)) th
+ETA_CONV
+ETA_RULE
+ETA
+*)
+
+(*
+val () = use "/home/ramana/HOL/src/tfl/src/RW.sml";
+val () = use "/home/ramana/HOL/src/tfl/src/Defn.sml";
+val () = RW.monitoring := true;
+*)
+
+(*
+fun GNOT_ABS_INVERSE_ETA_CONV t = let
+  val _ = assert (not o pairLib.is_pabs) t
+in
+  INVERSE_ETA_CONV (genvar(#1(dom_rng(type_of t)))) t
+end handle e => raise wrap_exn "" "GNOT_ABS_INVERSE_ETA_CONV" e
+
+fun VNOT_ABS_INVERSE_ETA_CONV s t = let
+  val _ = assert (not o pairLib.is_pabs) t
+  val vs = free_vars t
+in
+  INVERSE_ETA_CONV (prim_variant vs (mk_var (s,(#1(dom_rng(type_of t)))))) t
+end handle e => raise wrap_exn "" "VNOT_ABS_INVERSE_ETA_CONV" e
+
+fun VCOMB_INVERSE_ETA_CONV s t = let
+  val _ = assert is_comb t
+  val vs = free_vars t
+in
+  INVERSE_ETA_CONV (prim_variant vs (mk_var (s,(#1(dom_rng(type_of t)))))) t
+end handle e => raise wrap_exn "" "VCOMB_INVERSE_ETA_CONV" e
+*)
+
+
+(* Conversions for selectively applying (inverse) eta on certain constants *)
+
+fun UNETA_CONV x t =
+  let val (dom,rng) = dom_rng (type_of t)
+      val tysubst = [alpha |-> dom, beta |-> rng]
+      val th = SYM (SPEC t (INST_TYPE tysubst ETA_AX))
+      val tm = mk_abs (x,(mk_comb(t,x)))
+  in
+    TRANS th (ALPHA (rhs (concl th)) tm)
+  end
+  handle e => raise wrap_exn "" "UNETA_CONV" e
+
+fun UNETA_THESE_CONV ts x t = let
+  val (rator,_) = strip_comb t
+  val _ = assert (exists (can (C match_term rator))) ts
+in
+  UNETA_CONV x t
+end handle e => raise wrap_exn "" "UNETA_THESE_CONV" e
+
+fun ETA_THESE_CONV ts t = let
+  val (rator,_) = strip_comb (#2(dest_abs t))
+  val _ = assert (exists (can (C match_term rator))) ts
+in
+  ETA_CONV t
+end handle e => raise wrap_exn "" "ETA_THESE_CONV" e
+
+local
+  (* Insert all definitions required to get Defn.parse_from_absyn here.
+     Alternatively just expose parse_from_absyn, or put a version of Hol_defn
+     that takes a list of terms to uneta into Defn.
+
+     Would actually need Defn.parse_quote in order to deal with multiple
+     definitions at once (for mutual recursion). *)
+  val ERRloc = mk_HOL_ERRloc "myDefn"
+
+  local fun underscore #"_" = true  | underscore   _  = false
+  in
+  fun wildcard s =
+    let val ss = Substring.full s
+    in if Substring.isEmpty ss then false
+       else Substring.isEmpty (Substring.dropl underscore ss)
+    end
+  end
+
+  fun vary s S =
+   let fun V n =
+        let val s' = s^Lib.int_to_string n
+        in if mem s' S then V (n+1) else (s',s'::S)
+        end
+   in V 0 end
+
+  local
+    val v_vary = vary "v"
+    fun tm_exp tm S =
+      case dest_term tm
+      of VAR(s,Ty) =>
+           if wildcard s then
+             let val (s',S') = v_vary S in (Term.mk_var(s',Ty),S') end
+           else (tm,S)
+       | CONST _  => (tm,S)
+       | COMB(Rator,Rand) =>
+          let val (Rator',S')  = tm_exp Rator S
+              val (Rand', S'') = tm_exp Rand S'
+          in (mk_comb(Rator', Rand'), S'')
+          end
+       | LAMB _ => raise ERR "tm_exp" "abstraction in pattern"
+    open Absyn
+  in
+  fun exp (AQ(locn,tm)) S =
+        let val (tm',S') = tm_exp tm S in (AQ(locn,tm'),S') end
+    | exp (IDENT (p as (locn,s))) S =
+        if wildcard s
+          then let val (s',S') = v_vary S in (IDENT(locn,s'), S') end
+          else (IDENT p, S)
+    | exp (QIDENT (p as (locn,s,_))) S =
+        if wildcard s
+         then raise ERRloc "exp" locn "wildcard in long id. in pattern"
+         else (QIDENT p, S)
+    | exp (APP(locn,M,N)) S =
+        let val (M',S')   = exp M S
+            val (N', S'') = exp N S'
+        in (APP (locn,M',N'), S'')
+        end
+    | exp (TYPED(locn,M,pty)) S =
+        let val (M',S') = exp M S in (TYPED(locn,M',pty),S') end
+    | exp (LAM(locn,_,_)) _ = raise ERRloc "exp" locn "abstraction in pattern"
+
+  fun expand_wildcards asy (asyl,S) =
+     let val (asy',S') = exp asy S in (asy'::asyl, S') end
+  end
+
+  local open Absyn
+  in
+  fun vnames_of (VAQ(_,tm)) S = union (map (fst o Term.dest_var) (all_vars tm)) S
+    | vnames_of (VIDENT(_,s)) S = union [s] S
+    | vnames_of (VPAIR(_,v1,v2)) S = vnames_of v1 (vnames_of v2 S)
+    | vnames_of (VTYPED(_,v,_)) S = vnames_of v S
+
+  fun names_of (AQ(_,tm)) S = union (map (fst o Term.dest_var) (all_vars tm)) S
+    | names_of (IDENT(_,s)) S = union [s] S
+    | names_of (APP(_,IDENT(_,"case_arrow__magic"), _)) S = S
+    | names_of (APP(_,M,N)) S = names_of M (names_of N S)
+    | names_of (LAM(_,v,M)) S = names_of M (vnames_of v S)
+    | names_of (TYPED(_,M,_)) S = names_of M S
+    | names_of (QIDENT(_,_,_)) S = S
+  end
+
+  local
+    fun dest_pvar (Absyn.VIDENT(_,s)) = s
+      | dest_pvar other = raise ERRloc "munge" (Absyn.locn_of_vstruct other)
+                                       "dest_pvar"
+    fun dest_atom tm = (dest_const tm handle HOL_ERR _ => dest_var tm);
+    fun dest_head (Absyn.AQ(_,tm)) = fst(dest_atom tm)
+      | dest_head (Absyn.IDENT(_,s)) = s
+      | dest_head (Absyn.TYPED(_,a,_)) = dest_head a
+      | dest_head (Absyn.QIDENT(locn,_,_)) =
+              raise ERRloc "dest_head" locn "qual. ident."
+      | dest_head (Absyn.APP(locn,_,_)) =
+              raise ERRloc "dest_head" locn "app. node"
+      | dest_head (Absyn.LAM(locn,_,_)) =
+              raise ERRloc "dest_head" locn "lam. node"
+    fun strip_tyannote0 acc absyn =
+        case absyn of
+          Absyn.TYPED(locn, a, ty) => strip_tyannote0 ((ty,locn)::acc) a
+        | x => (List.rev acc, x)
+    val strip_tyannote = strip_tyannote0 []
+    fun list_mk_tyannote(tyl,a) =
+        List.foldl (fn ((ty,locn),t) => Absyn.TYPED(locn,t,ty)) a tyl
+  in
+  fun munge eq (eqs,fset,V) =
+   let val (vlist,body) = Absyn.strip_forall eq
+       val (lhs0,rhs)   = Absyn.dest_eq body
+       val   _          = if exists wildcard (names_of rhs []) then
+                           raise ERRloc "munge" (Absyn.locn_of_absyn rhs)
+                                        "wildcards on rhs" else ()
+       val (tys, lhs)   = strip_tyannote lhs0
+       val (f,pats)     = Absyn.strip_app lhs
+       val (pats',V')   = rev_itlist expand_wildcards pats
+                              ([],Lib.union V (map dest_pvar vlist))
+       val new_lhs0     = Absyn.list_mk_app(f,rev pats')
+       val new_lhs      = list_mk_tyannote(tys, new_lhs0)
+       val new_eq       = Absyn.list_mk_forall(vlist, Absyn.mk_eq(new_lhs, rhs))
+       val fstr         = dest_head f
+   in
+      (new_eq::eqs, insert fstr fset, V')
+   end
+  end
+
+  fun elim_wildcards eqs =
+   let val names = names_of eqs []
+       val (eql,fset,_) = rev_itlist munge (Absyn.strip_conj eqs) ([],[],names)
+   in
+     (Absyn.list_mk_conj (rev eql), rev fset)
+   end
+
+  fun parse_absyn absyn0 =
+   let val (absyn,fn_names) = elim_wildcards absyn0
+       val restore_these = map (fn s => (s, Parse.hide s)) fn_names
+       fun restore() =
+         List.app (fn (s, data) => Parse.update_overload_maps s data)
+                  restore_these
+       val tm  = Parse.absyn_to_term (Parse.term_grammar()) absyn
+                 handle e => (restore(); raise e)
+   in
+     restore();
+     (tm, fn_names)
+   end
+in
+  fun qrule ts x q = let
+    val (t,_) = parse_absyn (Parse.Absyn q)
+    fun term_to_quote t = [QUOTE (term_to_string t) : term frag]
+    val th = DEPTH_CONV (UNETA_THESE_CONV ts x) t handle UNCHANGED => REFL t
+    val t = rhs (concl th)
+  in
+    term_to_quote t
+  end
+  fun unconv_rule ts = CONV_RULE (DEPTH_CONV (ETA_THESE_CONV ts))
+end
+
+val state_option_consts =
+[``STATE_OPTION_BIND``,
+ ``STATE_OPTION_IGNORE_BIND``,
+ ``STATE_OPTION_UNIT`` ];
+
+(* Define foo using the quote the user wants to write. But the user must use
+qrule and know the constants to pass, and the (type of the) variable to use  *)
+val foo_defn = Defn.Hol_defn "foo" (
+qrule state_option_consts ``s:'a`` `
+foo M =
   STATE_OPTION_BIND (STATE_OPTION_UNIT F)
   (λb. STATE_OPTION_IGNORE_BIND
          (if b then foo M else STATE_OPTION_UNIT ())
-         (STATE_OPTION_UNIT ()))`
-(WF_REL_TAC `REMPTY` >> srw_tac [][STATE_OPTION_UNIT_def]);
+         (STATE_OPTION_UNIT ()))`);
+(* prove the termination goal *)
+val p = Defn.tprove (foo_defn,
+WF_REL_TAC `REMPTY` >>
+srw_tac [][STATE_OPTION_UNIT_def]);
+(* extract the theorems the user wants to see *)
+val (foo_def,foo_ind) = W (curry op ##) (unconv_rule state_option_consts) p;
 
-Hol_defn "plen" `
+(* Same procedure works for this example.
+A separate bug is that you can't remove the s argument from both sides of this
+quote. *)
+val ignore_rec_defn = Defn.Hol_defn "ignore_rec" (
+qrule state_option_consts ``s:'a`` `
+  ignore_rec s = STATE_OPTION_IGNORE_BIND
+                 (λs. OPTION_MAP (combin$C $, s) (OPTION_GUARD (s T)))
+                 (λs. ignore_rec ((T =+ ¬(s T)) s))
+                 s`);
+val p = Defn.tprove (ignore_rec_defn,
+WF_REL_TAC `measure (λs. if s T then 1 else 0)` >>
+srw_tac [][combinTheory.APPLY_UPDATE_THM,OPTION_GUARD_def]);
+val (ignore_rec_def,ignore_rec_ind) =
+W (curry op ##) (unconv_rule state_option_consts) p;
+
+val plen_defn = Defn.Hol_defn "plen" (
+qrule state_option_consts ``s:state`` `
   plen M = do
     (λs. STATE_OPTION_LIFT (OPTION_GUARD (∃ls. list_of_List embed_Term s M ls)) s) ;
     b <- EmptyListOfTerms M ;
@@ -19,7 +319,30 @@ Hol_defn "plen" `
       plen M
     od else return 0 ;
     return (n + 1)
-  od`
+  od`)
+val p = Defn.tprove (plen_defn,
+(* I haven't proved termination here yet, because it's a lot more difficult
+here, but I am semi-confident that the termination goal is (at last) provable
+*)
+)
+val (plen_def,plen_ind) =
+W (curry op ##) (unconv_rule state_option_consts) p;
+
+(* You can then use save_thm to save the right form of the definition and
+induction. There are no extra flags or tags necessary to completely emulate
+Define, right? *)
+
+(*
+val fail = Hol_defn "ignore_rec" Term`
+  ignore_rec = STATE_OPTION_IGNORE_BIND
+                 (λs. OPTION_BIND (FLOOKUP s 0)
+                       (OPTION_MAP (C $, s) o OPTION_GUARD o ($<> 0)))
+                 (λs. ignore_rec (s |+ (0, s ' 0 - 1)))`;
+
+val _ = Hol_defn "foo0" `foo0 = (λs. s ≠ 0 ∧ foo0 (s - 1))`;
+val _ = Hol_defn "foo1" `foo1 x = (λs. s ≤ x ∧ foo1 x (SUC s))`;
+*)
+
 (*
 val STATE_OPTION_GET_def = Define`
   STATE_OPTION_GET : ('a,'a) state_option
